theories/Compositional_Structures/Basic_Modules/Component_Types/Social_Choice_Types/List_Refine_Complete.thy
@@ -50,7 +50,7 @@ proof (unfold pl_\<alpha>_def, safe, clarsimp_all, safe)
   from tupler lor have aA: "a \<in> A"
     unfolding linear_order_on_def partial_order_on_def preorder_on_def refl_on_def
     by blast
-  from lol have "set l = A" unfolding losimp by simp
+  from lol have "set l = A" unfolding lin_order_equiv_A by simp
   from aA this show "a \<in> set l" by simp
 next
   fix a b :: 'a
@@ -58,12 +58,12 @@ next
   from tupler lor have aA: "b \<in> A"
     unfolding linear_order_on_def partial_order_on_def preorder_on_def refl_on_def
     by blast
-  from lol have "set l = A" unfolding losimp by simp
+  from lol have "set l = A" unfolding lin_order_equiv_A by simp
   from aA this show "b \<in> set l" by simp
 next
   fix a b :: 'a
   assume tupler: "(a, b) \<in> r"
-  from lol have Al: "set l = A" unfolding losimp by simp
+  from lol have Al: "set l = A" unfolding lin_order_equiv_A by simp
   from tupler lor have aA: "a \<in> A"
     unfolding linear_order_on_def partial_order_on_def preorder_on_def refl_on_def
     by blast
@@ -95,7 +95,7 @@ next
   assume al: "a \<in> set l"
   assume bl: "b \<in> set l"
   assume icmp: "index l b \<le> index l a"
-  from lol have Al: "set l = A" unfolding losimp by simp
+  from lol have Al: "set l = A" unfolding lin_order_equiv_A by simp
   from al bl have eitheror: "(a,b) \<in> r \<or> (b,a) \<in> r"
     using lor
     unfolding Al linear_order_on_def total_on_def
@@ -153,7 +153,7 @@ next
   from lobaro have lobalo: "linear_order_on_l F balo"
     using balrel linearorder_ref[THEN fun_relD, THEN fun_relD]
     by auto
-  then have seteqo: "set balo = F" unfolding losimp by simp
+  then have seteqo: "set balo = F" unfolding lin_order_equiv_A by simp
   from ih(1) have finxF: "finite (insert x F)"
     by simp
   from ih.prems have nempcons: "{b. (x, b) \<in> bar} \<noteq> {}"
@@ -206,7 +206,7 @@ next
     unfolding limit_l.simps defnb fdx append_take_drop_id
     by simp
   have lonb: "linear_order_on (insert x F) (pl_\<alpha> newbal)"
-    using seteqnb[symmetric] unfolding losimp[symmetric] 
+    using seteqnb[symmetric] unfolding lin_order_equiv_A[symmetric] 
    linord_eq . 
   have barolim: "baro = limit F (pl_\<alpha> newbal)"
     using limit_eq[where bal=newbal and A = F] disnb
